diffeq
=====

- Category: math
- Tags: arsenau
- Created: 2025-09-02 @ 12:52:44-4:00

Section 2.1
---

1.

   $$
   F = MA
   $$

2.

   $$
   A = P - K\,V
   $$

where \(P\) is the initial acceleration (≈ 11.0 for Usain), \(V_{\max}\) is max velocity (≈ 12.2 for Usain), and \(K\) depends on the person.

So we could find \(k = 11/12.2\). Using (1) and (2),
$$
MA = MP - MKV,
$$
let \(A = V'\). Usain equation:
$$
V' + \frac{11}{12.2} V = 11.0.
$$

This is a first-order linear ODE.

General form:
$$
v' + K v = P.
$$

Integrating factor:
$$
\mu(t) = e^{Kt}.
$$

Distribute the integrating factor:
$$
(e^{Kt} v)' = P\,e^{Kt}.
$$

Integrate both sides:
$$
v(t) = \frac{P}{K} + C e^{-K t}.
$$

For Usain:
$$
V(t) = 12.2 + C\,e^{-(11/12.2)t}.
$$

Now let \(p(t), q(t)\) be non-constants:
$$
y' + p(t)\,y = q(t), \qquad \mu(t) = e^{\int p(t)\,dt}.
$$
Multiply by \(\mu(t)\):
$$
\mu(t) y' + \mu(t) p(t) y = \mu(t) q(t).
$$
Take derivative (product rule):
$$
(\mu(t) y)' = \mu(t) q(t),
$$
so
$$
y(t) = \frac{1}{\mu(t)}\!\left(\int \mu(t)\,q(t)\,dt + C\right).
$$

Section 2.2 further discussions on linear First ODE
---
$$
\text{Theorem: if } p(t), q(t) \text{are continuous on an open interval containing } t=t_{0} \text{ then } \exists \text{ a unique soln, s.t. } y(t_{0})=y_{0}
$$


$$
y'+p(t)y=q(t)
$$

Ex1

$$
y' = \frac{4t^2-2y}{t}
$$

$$
y'+\frac{2}{t}y=4t
$$
$$
e^{ \int \frac{2}t \, dt  } =t^2
$$

$$
\int \frac{d}{dt}(t^2y)dt=\int 4t^{3}dt
$$

$$
\text{ we get: } t= \frac{t^4+c}{e^{ 2 }}=t^2+ct^{2}
$$

Ex2

$$
y'+\frac{2(1+t)}{t(2+t)}y=\frac{1+3t^2}{t(2+t^{2})} \text{ and } y(-1)=1
$$

need to use partial fractions here: 

$$
\int \frac{A}{t}+\frac{B}{t+2}dt = e^{ \ln|t|+\ln|t+2| }
$$

$$
\text{giving } I(t) = t(t+2)
$$

 solve the integrating factor problem

$$
y= \frac{t+t^{3}+c}{t(t+2)}
$$

plug in our initial condition,  giving

$$ 
c=1 
$$



2.3 -- Separable differential equation
---

$$
\frac{dy}{dx} = F(x,y)
$$

translated into

$$
M(x)dx + N(y)dy = 0
$$
or 

$$
M(x)+N(y)\cdot \frac{dy}{dx}=0
$$

EX 1:
$$
\frac{dy}{dx} = \frac{3x^2+1}{3y^2-6y}
$$
$$
\int(3y^2-6y) dy=\int(3x^2+1)dx
$$
$$
y^3-3y^2=x^{3}+x+C
$$

note that 
$$
y \neq 0, 2
$$
so interval is
$$
(0,2) \lor (-\infty, 0) \lor (2,\infty)
$$

EX2
a) find the solution Eq. 
b) given y(1) = -2, find the solution eq
c) given y(1) = 4, write a solution eq

$$
\frac{dy}{dx} =\frac{1-2x}{y}
$$

$$
\text{a)} \quad \int ydy = \int(1-2x)dx
$$
$$
\frac{1}{2}y^2= x-x^2+C
$$

$$
\text{b)} \quad \frac{1}{2}\cdot 4 = C
$$

$$
\text{b)} \quad \frac{1}{2}\cdot 16 = C
$$


2.8.1 exact equations
---

$$
M(x,y) + N(x,y) \cdot y' = 0
$$

$$
\text{Find: } \psi(x,y) = c 
$$
such that
$$
\frac{\partial \psi}{\partial x} =M(x,y)
$$
and
$$
\frac{\partial \psi}{\partial y} =N(x,y)
$$
so
$$
\frac{\partial \psi}{\partial x} + \frac{\partial \psi}{\partial y} \cdot \frac{dy}{dx} =0
$$

Clairaut's THM: taking the partial derivative wrt x and then also taking it wrt y, it's the same as vice versa

so if
$$
\frac{\partial M}{\partial y} =\frac{\partial N}{\partial x}
$$
then our og equation is an exact equation 


EX1
$$
\frac{y}{x} + 6x + (\ln x-2)  \frac{dy}{dx} = 0 
$$

(dy dx coudl be seperated out a first, doesnt matter as long as we can get to this form)

take the partial derivative wrt y on LHS
$$
\frac{\partial M}{\partial Y}= \frac{1}{x}
$$take the partial derivative wrt x on RHS

$$
\frac{\partial M}{\partial Y}= \frac{1}{x}
$$

again on LHS
$$
\int \frac{y}{x}+6x\text{ } dx
$$
giving: 
$$
y\ln x + 3x^2
+C(y)
$$
now derive this wrt y
$$
\ln x + C'(y)
$$
now we set C'(y) to any function with no x's in it????
$$
C'(y) = -2 \quad C(y) = -2y + C

$$
and on RHS

$$
\int \ln x -2 \text{ } dy
$$
giving; 
$$
y\ln x -2y + C(x)
$$

$$
\frac{y}{x} + D'(x) 
$$
D can be any function
$$
D'(x) = 6x 
$$
$$
D(x) = 3x^2 + C
$$

plug D into our integrated function
$$
\Psi (x, y) \implies y\ln|x| + 3x^2 - 2y = C
$$

explicitly 
$$
y = \frac {C-3x^2}{\ln x - 2}
$$



2.8.2 Integrating Factors to create an Exact equation 
---

$$
M (x,y) dx + N(x,y)dy = 0
$$
unfortuntately, we find this equation is not exact, using method from 2.8.1

so wtf integrating factor
$$
\mu(x,y)
$$
$$
\mu(x,y) M(x,y)dx + \mu(x,y)N(x,y)dy = 0
$$
this is Exact iff

$$
\frac{\partial}{\partial y} (\mu \cdot M) = \frac{\partial}{\partial x} (\mu \cdot N)
$$

$$
\mu \cdot M_{y} + M_{}{y} \cdot \mu = \mu_{x} \cdot N + \mu \cdot N_{x}
$$

$$
\mu(M_{y} -N_{x}) =M_{x}N - M_{y} N
$$

still too diff to solve, let's look at some specfic cases
solve if mu is some function of only one variable

$$
\text{if } \mu=f(x) \text{ then } \mu_{y} = 0
$$
$$
\mu_{x} = \frac{\mu (M_{y} -N_{x})}{N}
$$
solveable differential equation
$$
\frac{ (M_{y} -N_{x})}{N} = g(x)
$$

cliffhanger, will solve tmr 


the derivative of integrating factor is either 
$$
(\frac{N_{x}-M_{y}}{M})\cdot \mu
$$
in terms of y, 
or the oppositish thing in terms of x



2.9 Homogenous Eqs.
---

$$
\frac{dy}{dx}
$$
is homogenous when it doesnt depend on x or y
but instead y/x or x/y

$$
\text{If } \frac{dy}{dx}=F\left( \frac{y}{x} \right) , \text{then let } y= vx  \text{ or } v = \frac{y}{x}
$$

$$
v+\frac{dv}{dx} \cdot x = F(v)
$$
$$
\frac{dy}{dx} = v + \frac{dv}{dx} \cdot x
$$
remember we can switch x and y for everything when we see 
$$
F\left( \frac{x}{y} \right)
$$

Ex
$$
(x^{2} + 3xy + y^{2})dx = x^{2} dy
$$
$$
\left( 1+\frac{3y}{x} + \left( \frac{y}{x} \right)^2\right) = \frac{dy}{dx} 
$$
replace y/x with v
$$
(1+3v+v^{2})=v+\frac{dv}{dx} \cdot x
$$
$$
1+2v+v^{2} = \frac{dv}{dx} \cdot x
$$

$$
(v+1)^{2} = \frac{dv}{dx} \cdot x
$$
$$
\frac{dx}{x} = \frac{dv}{(v+1)^2}
$$

$$
\ln|x|+c =-\frac{1}{v+1}
$$
solve for v

$$
-\frac{1}{\ln|x| +c} = v + 1
$$
$$
\frac{y}{x} = v = -\frac{1}{\ln|x|+c}
$$
$$
y = -\frac{x}{\ln|x| + c} - x
$$

the slopefield of a homogenous equation is always symmetrical about the origin

all homogenous equations have equillibrium points. 