3.2 Fundamental Solutions of Linear Homogenous Eqs Linear independence and the Wronskin
=====
- Category: 
- Tags: 
- Created: 2025-09-24 @ 13:01:09-4:00

$$
y'' + p(t) y' + q(t) =g(t)
$$

$$
\exists \text{ a unique solution s.t. that soln is twice diferentiable on an interval } t \in (a,b)
$$

EX:

$$
(t^{2} - 3t ) y'' + ty' - (t+3) y = 0
$$
$$
y(1) = 2 , y' (1) =1

$$
because we have to isolate y''
$$
t \neq 0, \, t \neq 3
$$
and so 
$$
\exists \text{ a unique soln in the interval } t \in (0,3)
$$

generally; 

$$
\begin{matrix}
\text{when } y_{1}(t) \text{and } y_{2}(t)\text{ are solutions of } y'' py' + qy = 0   \\
\text{then } y= c_{1} y_{1} (t) + c_{2}y_{2}(t) \text{is a solution }
\end{matrix}
$$

so we can get 

$$
c_{1}y_{1}(t_{0}) + c_{2}y_{2}(t_{0}) = y_{0} \text{ and }  c_{1}y'_{1}(t_{0}) + c_{2}y'_{2}(t_{0}) = y'_{0} 
$$
using cramer's rule

$$
C_{1} = \frac{\det \left| \begin{matrix}
 y_{0}  & y_{2}(t_{0})  \\
 y'0 & y_{2}'(t_{0})
\end{matrix} \right| }{ \det \left| \begin{matrix}
y_{1}(t_{0} )& y_{2}(t_{0})  \\
y'_{1}(t_{0}) & y'_{2}(t_{0}) 
\end{matrix} \right| }
$$
and 
$$
\det \left| \begin{matrix}
y_{1}(t_{0} )& y_{2}(t_{0})  \\
y'_{1}(t_{0}) & y'_{2}(t_{0}) 
\end{matrix} \right|  =W
$$
where W is the wronskian 

so 
$$
C_{2} = \frac{\left| \begin{matrix}
y_{1} (t_{0} ) & y_{0}  \\
y_{1}' (t_{0}) & y'_{0}
\end{matrix} \right| }{W}
$$

THM 3.2.3

$$
W = y_{1}y_{2}' - y_{1}' y_{2} \neq 0
$$
$$
\begin{matrix}
\text{for } y(t_{0} ) = y_{0}  \\
y' (t_{0} ) = y'_{0} \\
 \\
\exists \text{ a linear combinaton that satisfies the Diff Eq}
\end{matrix} 
$$

THM 3.2.4

$$
W \neq 0 
$$

$$
\text{arbitrary values of } C_{1} \text{ and }  C_{2} \text{ create every possible solution of the Diffeq}
$$

EX:
$$
\left[  \begin{matrix}
y_{1} \text{ is a solution s.t. }y_{1}(t_{0}) = 1, y_{1}' (t_{0}) = 0 \\
y_{2} \text{ is a solution s.t. }y_{2}(t_{0}) = 1, y_{2}' (t_{0}) = 1
\end{matrix} \right] 
$$

$$
y '' -y = 0 
$$

$$
r^{2}-1 = 0 
$$

$$
r=\pm 1
$$
$$
y = C_{1}e^t + C_{2}e^{-t}
$$
from y = 1
$$
1 = C_{1} + C_{2}
$$
from y' = 0
$$
0 = C_{1} - C_{2}
$$
so 
$$
C_{1} = C_{2} = \frac{1}{2}
$$
now make two functions  
$$
\begin{matrix}
y_{1} = \frac{1}{2 }e^t + \frac{1}{2 }e^{-t} = \frac{e^{ t } + e^{ -t}}{2} = \cosh t
 \\
y_{2} = \frac{1}{2 }e^t - \frac{1}{2 }e^{-t} = \frac{e^{ t } - e^{ -t}}{2} = \sinh t
\end{matrix}
$$

$$
y = C_{1}\cosh t + C_{2} \sinh t
$$

note that

$$
\cosh ^{2}t - \sinh ^{2} t = 1 \neq 0 
$$
thf

$$
\exists \text{ a  family of solutions using } C_{1} \text{ and } C_{2}
$$

$$

$$
