3.4 2nd Order Homogenous DiffEq w/ Complex Roots
=====
- Category: 
- Tags: 
- Created: 2025-09-26 @ 10:40:06-4:00


given

$$
Ay'' + By' + Cy = 0 \quad y = e^{rt}
$$

then
$$
r_{1} = a+bi \quad r_{2} = a=bi
$$

$$
y = c_{1}e^{(a+bi)t} + c_{2} e^{(a-bi)t}
$$

$$
e^{it} = 1+it -\frac{t^2}{2!} -\frac{it^3}{3!}+. . .+ . . .- . . .
$$

$$
\cos t = 1- \frac{t^2}{2!} + \frac{t^4}{4!} + . . .
$$

$$
i\sin t = i\left( t-\frac{t^3}{3!} + \frac{t^5}{5!}+ . . . \right)
$$

so 

$$
y = c_{1}e^{at} (\cos bt + i\sin bt ) + c_{2}e^{at} (\cos bt - i \sin bt)
$$

let c1 = 1 , c2 = 0
we just get the first term
$$
y = c_{1}e^{at} (\cos bt + i\sin bt ) 
$$

let c2 = 1 , c1 = 0
we just get the second term 

$$
c_{2}e^{at} (\cos bt - i \sin bt)

$$

$$
y_{1} + y_{2} = 2e^{at} \cos bt
$$

when c1 = i  and c2 = i 

$$
y_{1} - y_{2} = 2e^{at} \sin bt
$$
(i's cancel from within the parentese and the cs)

using our two soln groups

$$
y_{3} = c_{1}e^{at } \cos bt \quad y_{4} = c_{2} e^{at} \sin bt
$$
finally giving

$$
y = e^{at }(c_{1}\cos bt + c_{2} \sin bt)
$$

solving the wronskian for y


$$
be^{ 2at } \neq 0 
$$


Ex

$$
\begin{matrix}

y'' + 2y' + 2y = 0  \\
r^{2} + 2r + 2 =0  \\

r = \frac{-2 \pm 2i}{2} = -1 \pm i \\

 y = e^{ -t } (c_{1}\cos t + c_{2} \sin t) \\ \\
\text{let } y'\left( \frac{\pi}{4}\right) = -2  \\
y\left( \frac{\pi}{4}\right) = -2  \\ \\
\text{ solve for constants}

\end{matrix}

$$



when is it possible to change  ahomogenous Diff Eq to a 2nd order with constant coefficient via substitution. 


$$
y'' + p(t)y' + q(t)y = 0
$$

$$
\text{where } x=f(t) 
$$


$$
y' = \frac{dy}{dt} = \frac{dy}{dx} \cdot \frac{dx}{dt}
$$

$$
y'' = \frac{d}{dt}(y') = \frac{d^{2}y}{dx^{2}}\cdot \frac{dx}{dt} \cdot \frac{dx}{dt} + \frac{dy}{dx} \cdot \frac{d^{2}x}{dt^{2}}
$$

so going back to standard form:

$$
\frac{dy}{dx}\cdot \frac{d^{2}x}{dt^{2}}+\frac{d^{2}y}{dt}\left( \frac{dx}{dt} \right)^2+p(t)  \frac{dy}{dx} \cdot \frac{dx}{dt} + q(t) y=0
$$

factor:

$$
\frac{d^{2}y}{dx^{2}}\left( \frac{dx}{dt} \right)^{2} + \frac{\left( \frac{d^{2}x}{dt^{2}}+p \frac{dx}{dt} \right)dy}{dx} + q(t)y = 0
$$

so now using y as a function of x..

$$
y'' + \left( \frac{\frac{d^{2}x}{dt^{2}}+{\frac{dx}{dt}p}}{\left( \frac{dx}{dt} \right)^2} \right) + \frac{q}{\left( \frac{dx}{dt} \right)^2}y = 0
$$

let the coeffecient of y = 1

use algebra to get

$$
\frac{dx}{dy} = q(t)^{\frac{1}{2}}
$$

$$
\frac{d^{2}x}{dt^{2}} = \frac{1}{2} (q(t)^{-\frac{1}{2}}\cdot g'(t))
$$

$$
x = \int q(t)^{1/2} \, dt
$$
solving this:

$$
\text{coeff of } y'= \frac{q'+2qp}{2q^{3/2}} 
$$



