3.5 Repeated Roots
=====
- Category: 
- Tags: 
- Created: 2025-10-01 @ 14:20:29-4:00

$$
ay'' + by' +cy =0
$$

$$
e^{ rt }(ar^{2} + br + C)= 0 
$$

say you have a double root r

$$
y = c_{1}e^{ rt } + c_{2}e^{ rt }
$$

which is not linerarly independent 


let

$$
y = c_{1}e^{ rt } + c_{2}te^{ rt }
$$

which IS linearly independent.

but how to prove this??

$$
y'  = c_{1}re^{ rt } + c_{2}e^{ rt }+c_{2}re^{ rt }
$$


$$
y'' = c_{1}r^{2}e^{ rt } + 2c_{2}re^{ rt }+ c_{2}r^{2}te^{rt }
$$

plug back in

factor out c1e^rt and c2te^rt 

$$
c_{1}e^{ rt }(ar^{2}+br+c) + c_{2}e^{ rt }(2ar+b)+ c_{2}te^{ rt }(ar^{2}+br+c)=0
$$


the $$ 2ar + b$$ term is annoying

but notice that this is the tangent line to the equation at r. 

recall that for a double root the slope of the parabola is parallel to x axis meaning that the slope of the thing is r and it's also along the x axis so 

$$
a,b = 0
$$

so we are left with

$$
c_{1}e^{ rt }+c_{2}te^{ rt  }=0 
$$



EX: 

$$
\begin{matrix}
4y'' + 12y' + 9y = 0  \\
 \\
4r^{2} + 12r + 9 = 0 \\
 \\
r = \frac{{-12 \pm \sqrt{ 144-144 }}}{8} = -\frac{3}{2}\\
  \\
y = c_{1}e^{-\frac{3}{2}t   } + c_{2}te^{ -\frac{3}{2}t }

\end{matrix}
$$