3.6 Non-Homogenous Equations
=====
- Category: 
- Tags: 
- Created: 2025-10-06 @ 13:37:25-4:00


$$
y'' + (t)y' +q(t)y = g(t)
$$

$$
ay'' + by' + cy = g(t)
$$

note g is not constant anymore

$$
y = c_{1}e^{ r_{1}t }+c_{2}e^{ r_{2} t}

$$

guidelines for g

if
$$
g = e^{ 3t } \text{ try } y_{p} = Ae^{ 3t } 
$$
$$
g = \text{ nth degree polynomial try } y_{p} =a_{n}t^n + a_{n-1}t^{n-1}\dots
$$
$$
\sin Kt \text{ and/or} \cos Kt \text{ try } y+p = A\sin kt + B\sin Kt
$$

$$
g = \text{product/sum of above try } y_{p} = \text{product/sum of the above} 
$$


the yc or complementary solution is basically the right side if the left side equals 0 
