14.4 Tangent Planes and Linearization
=====
- Category: 
- Tags: 
- Created: 2025-10-03 @ 13:14:26-4:00


so we know that

$$
z-z_{0} = f_{x} (x_{0},y_{0}) (x-x_{0}) + f_{y}(x_{0},y_{0})(y-y_{0})
$$

we can take this to make the lineariziation formula

$$
L(x,y) = f(a,b) +f_{x}(a,b)(x-a) + f_{y}(a,b)(y-b)
$$

$$
f(x,y) \text{ is the approximate value of f around } (a,b)
$$

Ex 

$$
z = x^{2} + xy + 3y^{2}
$$

where 

$$
x =1 , y= 1
$$

$$
\frac{\partial z}{\partial x} = 2x+  y = 3
$$

$$
\frac{\partial z}{\partial y}  = x+6y = 7
$$
using z
$$
f(1,1) = 5 = z
$$
the equation of the plane is

$$
z-5 = 3(x-1)+7(y-1)
$$


