14.5 The Chain Rule
=====
- Category: 
- Tags: 
- Created: 2025-10-07 @ 10:30:58-4:00


when 
$$
z = f(x,y) 
$$

is differentiable, where 

$$
x = g(t) \text{ and } y = h(t)
$$

are also diff


case1

then:

$$
\frac{dz}{dt} = \frac{{\partial z}}{\partial x} \cdot \frac{{dx}}{dt} + \frac{{\partial z}}{\partial y} \cdot \frac{dy}{dt}
$$
case2

$$
z = f(x,y) \dots \text{ where } x = g(r,s) \text{ and } y = h(r,s)
$$

$$
\frac{\partial z}{\partial r } = \frac{{\partial z}}{\partial x} \cdot \frac{{\partial x}}{\partial r} + \frac{{\partial z}}{\partial y} \cdot \frac{\partial y}{\partial r}
$$

and similar for dz ds



EX

Show:

$$
\frac{{\partial^{2}x}}{\partial x^{2}} + \frac{{\partial^{2}z}}{\partial y^{2}} = \frac{{\partial^{2}z}}{\partial r^{2}} + \frac{1}{r^{2}} \cdot \frac{{\partial^{2}z}}{\partial \theta^{2}} + \frac{1}{r} \frac{{\partial z}}{\partial r}
$$

Given 

$$
\begin{matrix}
z = f(x,y) \\
x = r\cos \theta \\
y = r\sin \theta
\end{matrix}
$$

draw the tree

$$
\frac{{\partial z}}{ \partial r} = \frac{{\partial z}}{\partial x} \cdot \frac{{\partial x}}{\partial r} + \frac{{\partial z}}{\partial y } \cdot \frac{{\partial y}}{ \partial r}
$$

$$
\frac{\partial x}{\partial r } = \cos \theta
$$

$$
\frac{{\partial y}}{\partial r} = \sin \theta
$$
so we can say 


$$
\frac{{\partial z}}{ \partial r} = \frac{{\partial z}}{ \partial x} \cdot \cos \theta + \frac{{\partial z}}{\partial y} \cdot \sin \theta
$$

now wtf 

$$
\frac{{\partial^{2}z}}{\partial r^{2}}
$$

$$
\frac{{\partial^{2}z}}{\partial r^{2}} = \frac{\partial}{\partial r} \left(  \frac{{\partial z}}{\partial x } \cos \theta + \frac{{\partial z}}{\partial y} \sin \theta \right) 
$$
first term of parenthesis

$$
\frac{{\partial^{2}z}}{\partial r^{2}}  = \frac{{\partial^{2}z}}{\partial x^{2}} \frac{{\partial x}}{\partial r}\cos \theta + \frac{{\partial^{2}z}}{\partial y\partial x} \cdot \frac{{\partial y}}{\partial r} \cos \theta
$$

second term

$$
+ \frac{{\partial^{2}z}}{\partial x\partial y} \cdot \frac{{\partial x}}{\partial r} \sin \theta + \frac{{\partial^{2}z}}{\partial y^{2}} \cdot \frac{{\partial y}}{\partial r}\sin \theta
$$

remember 

$$
\frac{\partial x}{\partial r} = \cos \theta
$$

so the derivative is
$$
\frac{{\partial^{2}z}}{\partial x^{2}} \cos ^{2}\theta + \frac{{\partial^{2}z}}{\partial y \partial x} \cos \theta \sin \theta + \frac{{\partial^{2}z}}{\partial x\partial y} \cos \theta \sin \theta + \frac{{\partial^{2}z}}{\partial y^{2}}\sin ^{2}\theta
$$

use clairauts:

$$
\frac{{\partial^{2}z}}{\partial x^{2}} \cos ^{2}\theta + 2 \cdot \frac{{\partial^{2}z}}{\partial y \partial x} \cos \theta \sin \theta  + \frac{{\partial^{2}z}}{\partial y^{2}}\sin ^{2}\theta
$$


next:

using the fact that

$$
\begin{matrix}
\frac{{\partial x}}{\partial \theta} = -r\sin \theta \\
\frac{{\partial y}}{\partial \theta} = r\cos \theta
\end{matrix}
$$

$$
\frac{{\partial z}}{\partial \theta} = -\frac{{\partial z}}{\partial x}r\sin \theta + \frac{{\partial z}}{\partial y}r\cos t\eta
$$

now for the double deriv:

$$
\frac{{\partial^{2}z}}{\partial \theta^{2}} = \frac{\partial}{ \partial \theta} \left(  - \frac{{\partial z}}{\partial x}\cdot r\sin \theta + \frac{{\partial z}}{\partial y}\cdot r\cos \theta \right) 
$$
term 1:

$$
=-\frac{{\partial z}}{\partial x} \cdot r\cos \theta - \frac{{\partial^{2}z}}{\partial x^{2}} \cdot \frac{{\partial x}}{{\partial \theta}}r\sin \theta - \frac{{\partial^{2}z}}{\partial y \partial x} \cdot \frac{{\partial y}}{\partial \theta}r\sin \theta
$$

term 2:

$$
-\frac{{\partial z}}{\partial y}r\sin \theta + \frac{{\partial^{2}z}}{\partial x \partial y} \frac{{\partial x}}{\partial \theta}r\cos \theta + \frac{{\partial^{2}z}}{\partial y^{2}} \cdot \frac{{\partial y}}{\partial \theta} r\cos \theta
$$
so 


$$
\frac{{\partial^{2} z}}{\partial \theta^{2}} = \left( -\frac{{\partial z}}{\partial x} r\cos \theta + \frac{{\partial^{2}z}}{\partial x^{2} }r^{2}\sin ^{2}\theta - \frac{{\partial^{2}z}}{\partial y\partial x}r^{2}\sin \theta \cos \theta -\frac{{\partial z}}{\partial y}r\sin \theta -\frac{{\partial^{2}z}}{\partial \partial x \partial y} r^{2} \sin \theta \cos \theta + \frac{{\partial^{2}z}}{\partial y^{2}} r^{2}\cos ^{2}\theta\right) 
$$

multiply this by 1/r^2

multiply the old thing by 1/r

add them

you'll prob get 

$$
\frac{{\partial^{2}z}}{\partial x^{2}} + \frac{\partial^{2}z}{\partial y^{2}}
$$


Implicit Differentiation

Ex:

$$
xyz = \cos(x+y + z)
$$
implied z = f(x,y)

$$
\text{find } \frac{{\partial z}}{\partial x}
$$

need to implicitly differentiate

$$
yz + xy \cdot \frac{{\partial z}}{\partial x} = - \sin (x+y+z) \left[  1 + \frac{{\partial z}}{\partial x} \right] 
$$
$$
\frac{{\partial z}}{\partial x}(xy + \sin(x+y+z) ) = -yz - \sin(x+y+z)
$$

$$
\frac{{\partial z}}{\partial x} = -\frac{yz+\sin(x+y+z)}{xy+\sin(x+y+z)}
$$

OR

you can let the whole thing = W

$$
W = xyz = \cos(x+y+z)
$$

xyz, now all independent


$$
W = xyz - \cos(x+y+z)
$$
need to solve

$$
\frac{\frac{{\partial w}}{\partial x}}{\frac{{\partial w}}{\partial z}} = -\frac{W_{x}}{W_{z}}
$$


which gives the same answer


